theories/lithium/interpreter.v
@@ -36,6 +36,7 @@ Ltac liUnfoldSyntax :=
   lazymatch goal with
   | |- envs_entails _ (li.all _) => liFromSyntax
   | |- envs_entails _ (li.exist _) => liFromSyntax
+  | |- envs_entails _ (li.and _ _) => liFromSyntax
   | |- envs_entails _ (li.done) => liFromSyntax
   | |- envs_entails _ (li.false) => liFromSyntax
   | |- envs_entails _ (li.bind0 _ _) => liFromSyntax
