tutorial/lithium/lang.v
@@ -1,0 +1,295 @@
+From stdpp Require Export strings binders.
+From lithium Require Export base.
+From iris.algebra Require Export ofe.
+From iris.program_logic Require Export language ectx_language ectxi_language.
+
+Open Scope Z.
+
+(* This language is inspired by simp-lang: https://github.com/tchajed/iris-simp-lang *)
+
+Definition prov : Set := Z.
+Definition loc : Set := prov * Z.
+
+Inductive base_lit :=
+  | LitInt (n : Z)
+  | LitLoc (l : loc).
+
+Definition NULL := LitInt 0.
+
+Inductive bin_op :=
+  | PlusOp
+  | MinusOp
+  | EqOp.
+
+Inductive un_op :=
+  | NegOp.
+
+Inductive expr :=
+  (* Values *)
+  | Val (v : val)
+  (* Base lambda calculus *)
+  | Var (x : string)
+  | Rec (f x : binder) (e : expr)
+  | App (e1 e2 : expr)
+  (* Pure operations *)
+  | BinOp (op : bin_op) (e1 e2 : expr)
+  | UnOp (op : un_op) (e : expr)
+  | If (e0 e1 e2 : expr)
+  | Assert (e : expr)
+  (* Heap *)
+  | Alloc (e1 : expr)
+  | Free (e1 e2 : expr)
+  | Load (e1 : expr)
+  | Store (e1 : expr)
+with val :=
+  | LitV (l : base_lit)
+  | RecV (f x : binder) (e : expr).
+
+Bind Scope expr_scope with expr.
+Bind Scope val_scope with val.
+
+
+Notation of_val := Val (only parsing).
+
+Definition to_val (e : expr) : option val :=
+  match e with
+  | Val v => Some v
+  | _ => None
+  end.
+
+Lemma to_of_val v : to_val (of_val v) = Some v.
+Proof. by destruct v. Qed.
+
+Lemma of_to_val e v : to_val e = Some v → of_val v = e.
+Proof. destruct e=>//=. by intros [= <-]. Qed.
+
+Global Instance of_val_inj : Inj (=) (=) of_val.
+Proof. intros ??. congruence. Qed.
+
+(** Instances *)
+Global Instance base_lit_eq_dec : EqDecision base_lit.
+Proof. solve_decision. Defined.
+Global Instance bin_op_eq_dec : EqDecision bin_op.
+Proof. solve_decision. Defined.
+Global Instance un_op_eq_dec : EqDecision un_op.
+Proof. solve_decision. Defined.
+Lemma expr_eq_dec (e1 e2: expr) : Decision (e1 = e2)
+with val_eq_dec (v1 v2 : val) : Decision (v1 = v2).
+Proof.
+  { refine
+      (match e1, e2 with
+        | Val v, Val v' => cast_if (decide (v = v'))
+        | Var x, Var x' => cast_if (decide (x = x'))
+        | Rec f x e, Rec f' x' e' => cast_if_and3 (decide (f = f')) (decide (x = x')) (decide (e = e'))
+        | App e1 e2, App e1' e2' | Free e1 e2, Free e1' e2' =>
+          cast_if_and (decide (e1 = e1')) (decide (e2 = e2'))
+        | BinOp op e1 e2, BinOp op' e1' e2' =>
+          cast_if_and3 (decide (op = op')) (decide (e1 = e1')) (decide (e2 = e2'))
+        | If e1 e2 e3, If e1' e2' e3' =>
+          cast_if_and3 (decide (e1 = e1')) (decide (e2 = e2')) (decide (e3 = e3'))
+        | UnOp op e, UnOp op' e' =>
+          cast_if_and (decide (op = op')) (decide (e = e'))
+        | Alloc e, Alloc e' | Load e, Load e' | Store e, Store e' | Assert e, Assert e' =>
+          cast_if  (decide (e = e'))
+        | _, _ => right _
+        end); solve [ abstract intuition congruence ]. }
+  { refine
+      (match v1, v2 with
+        | LitV l, LitV l' => cast_if (decide (l = l'))
+        | RecV f x e, RecV f' x' e' => cast_if_and3 (decide (f = f')) (decide (x = x')) (decide (e = e'))
+        | _, _ => right _
+        end); try solve [ abstract intuition congruence ]. }
+Defined.
+Global Instance expr_eq_dec' : EqDecision expr := expr_eq_dec.
+Global Instance val_eq_dec' : EqDecision val := val_eq_dec.
+
+Global Instance base_lit_countable : Countable base_lit.
+Proof.
+  refine (inj_countable'
+            (λ l, match l with | LitInt n => inl n | LitLoc l => inr l end)
+            (λ v, match v with | inl n => _ | inr l => _ end) _).
+  intros []; eauto.
+Qed.
+
+Global Instance bin_op_countable : Countable bin_op.
+Proof.
+  refine (inj_countable'
+            (λ op, match op with | PlusOp => 0 | MinusOp => 1 | EqOp => 2  end)
+            (λ n, match n with | 0 => _ | 1 => _ | 2 => _
+                          | _ => ltac:(constructor) end) _).
+  intros []; eauto.
+Qed.
+
+Global Instance un_op_countable : Countable un_op.
+Proof.
+  refine (inj_countable'
+            (λ op, match op with | NegOp => 0 end)
+            (λ n, match n with | 0 => _ | _ => ltac:(constructor) end) _).
+  intros []; eauto.
+Qed.
+
+(** Evaluation contexts *)
+Inductive ectx_item :=
+  | AppLCtx (v2 : val)
+  | AppRCtx (e1 : expr)
+  | BinOpLCtx (op : bin_op) (v2 : val)
+  | BinOpRCtx (op : bin_op) (e1 : expr)
+  | UnOpCtx (op : un_op)
+  | IfCtx (e1 e2 : expr)
+  | AssertCtx
+  | AllocCtx
+  | FreeLCtx (e2 : expr)
+  | FreeRCtx (v1 : val)
+  | LoadCtx
+  | StoreCtx.
+
+Definition fill_item (Ki : ectx_item) (e : expr) : expr :=
+  match Ki with
+  | AppLCtx v2 => App e (Val v2)
+  | AppRCtx e1 => App e1 e
+  | BinOpLCtx op v2 => BinOp op e (Val v2)
+  | BinOpRCtx op e1 => BinOp op e1 e
+  | UnOpCtx op => UnOp op e
+  | IfCtx e1 e2 => If e e1 e2
+  | AssertCtx => Assert e
+  | AllocCtx => Alloc e
+  | FreeLCtx e2 => Free e e2
+  | FreeRCtx v1 => Free (Val v1) e
+  | LoadCtx => Load e
+  | StoreCtx => Store e
+  end.
+
+(** Substitution *)
+Fixpoint subst (x : string) (v : val) (e : expr)  : expr :=
+  match e with
+  | Val _ => e
+  | Var y => if decide (x = y) then Val v else Var y
+  | Rec f y e =>
+    Rec f y $ if decide (BNamed x ≠ f ∧ BNamed x ≠ y) then subst x v e else e
+  | App e1 e2 => App (subst x v e1) (subst x v e2)
+  | BinOp op e1 e2 => BinOp op (subst x v e1) (subst x v e2)
+  | UnOp op e => UnOp op (subst x v e)
+  | If e0 e1 e2 => If (subst x v e0) (subst x v e1) (subst x v e2)
+  | Assert e => Assert (subst x v e)
+  | Alloc e => Alloc (subst x v e)
+  | Free e1 e2 => Free (subst x v e1) (subst x v e2)
+  | Load e => Load (subst x v e)
+  | Store e => Store (subst x v e)
+  end.
+
+Definition subst' (mx : binder) (v : val) : expr → expr :=
+  match mx with BNamed x => subst x v | BAnon => id end.
+
+(** Evaluation *)
+Definition LitBool (b:bool) : base_lit :=
+  if b then LitInt 1 else LitInt 0.
+
+Definition bin_op_eval (op : bin_op) (v1 v2: val) : option val :=
+  match op with
+  | PlusOp => match v1, v2 with
+              | LitV (LitInt n1), LitV (LitInt n2) =>
+                Some (LitV (LitInt (n1 + n2)))
+              | _, _ => None
+              end
+  | MinusOp => match v1, v2 with
+              | LitV (LitInt n1), LitV (LitInt n2) =>
+                Some (LitV (LitInt (n1 - n2)))
+              | _, _ => None
+              end
+  | EqOp => Some (LitV $ LitBool $ bool_decide (v1 = v2))
+  end.
+
+Definition un_op_eval (op: un_op) (v: val) : option val :=
+  match op, v with
+  | NegOp, LitV (LitInt n) => Some (LitV (LitInt (-n)))
+  | _, _ => None
+  end.
+
+(** state *)
+Record state : Type := {
+  heap: gmap loc val;
+}.
+
+Global Instance state_inhabited : Inhabited state :=
+  populate {| heap := inhabitant; |}.
+Global Instance val_inhabited : Inhabited val := populate (LitV (LitInt 0)).
+Global Instance expr_inhabited : Inhabited expr := populate (Val inhabitant).
+
+(** step relation *)
+Inductive observation :=.
+Lemma observations_empty (κs: list observation) : κs = [].
+Proof. by destruct κs as [ | [] ]. Qed.
+
+
+Inductive head_step : expr → state → list observation → expr → state → list expr → Prop :=
+  | RecS f x e σ :
+    head_step (Rec f x e) σ [] (Val $ RecV f x e) σ []
+  | BetaS f x e1 v2 e' σ :
+    e' = subst' x v2 (subst' f (RecV f x e1) e1) →
+    head_step (App (Val $ RecV f x e1) (Val v2)) σ [] e' σ []
+  | BinOpS op v1 v2 v' σ :
+    bin_op_eval op v1 v2 = Some v' →
+    head_step (BinOp op (Val v1) (Val v2)) σ [] (Val v') σ []
+  | UnOpS op v v' σ :
+    un_op_eval op v = Some v' →
+    head_step (UnOp op (Val v)) σ [] (Val v') σ []
+  | IfFalseS e1 e2 σ :
+    head_step (If (Val $ LitV $ LitInt 0) e1 e2) σ [] e2 σ []
+  | IfTrueS n e1 e2 σ :
+    0 ≠ n →
+    head_step (If (Val $ LitV $ LitInt n) e1 e2) σ [] e1 σ []
+  | AssertS n σ :
+    0 ≠ n →
+    head_step (Assert (Val $ LitV $ LitInt n)) σ [] (Val $ LitV $ LitInt 0) σ []
+(*  | AllocS v σ l :
+    σ.(heap) !! l = None →
+    head_step (HeapOp AllocOp (Val v) (Val $ LitV LitUnit)) σ
+              []
+              (Val $ LitV $ LitInt l) (state_upd_heap <[l := v]> σ)
+              []
+  | LoadS v σ l :
+    σ.(heap) !! l = Some v →
+    head_step (HeapOp LoadOp (Val $ LitV $ LitInt l) (Val $ LitV LitUnit)) σ
+              []
+              (Val $ v) σ
+              []
+  | StoreS v w σ l :
+    σ.(heap) !! l = Some v →
+    head_step (HeapOp StoreOp (Val $ LitV $ LitInt l) (Val $ w)) σ
+              []
+              (Val $ LitV $ LitUnit) (state_upd_heap <[l := w]> σ)
+              []
+*)
+.
+
+(** Properties for language interface *)
+
+Global Instance fill_item_inj Ki : Inj (=) (=) (fill_item Ki).
+Proof. destruct Ki; intros ???; simplify_eq/=; auto with f_equal. Qed.
+
+Lemma fill_item_val Ki e :
+  is_Some (to_val (fill_item Ki e)) → is_Some (to_val e).
+Proof. intros [v ?]. destruct Ki; simplify_option_eq; eauto. Qed.
+
+Lemma val_head_stuck e1 σ1 κ e2 σ2 efs : head_step e1 σ1 κ e2 σ2 efs → to_val e1 = None.
+Proof. destruct 1; naive_solver. Qed.
+
+Lemma head_ctx_step_val Ki e σ1 κ e2 σ2 efs :
+  head_step (fill_item Ki e) σ1 κ e2 σ2 efs → is_Some (to_val e).
+Proof. destruct Ki; inversion_clear 1; simplify_option_eq; eauto. Qed.
+
+Lemma fill_item_no_val_inj Ki1 Ki2 e1 e2 :
+  to_val e1 = None → to_val e2 = None →
+  fill_item Ki1 e1 = fill_item Ki2 e2 → Ki1 = Ki2.
+Proof. destruct Ki1, Ki2; naive_solver eauto with f_equal. Qed.
+
+Lemma tutorial_lang_mixin : EctxiLanguageMixin of_val to_val fill_item head_step.
+Proof.
+  split; apply _ || eauto using to_of_val, of_to_val, val_head_stuck,
+    fill_item_val, fill_item_no_val_inj, head_ctx_step_val.
+Qed.
+
+(** Language *)
+Canonical Structure tutorial_ectxi_lang := EctxiLanguage tutorial_lang_mixin.
+Canonical Structure tutorial_ectx_lang := EctxLanguageOfEctxi tutorial_ectxi_lang.
+Canonical Structure tutorial_lang := LanguageOfEctx tutorial_ectx_lang.
