tutorial/lithium/notation.v
@@ -1,0 +1,75 @@
+From lithium.tutorial Require Export lang.
+
+(* These notations are inspired by simp-lang: https://github.com/tchajed/iris-simp-lang *)
+
+(** Coercions to make programs easier to type. *)
+Coercion LitInt : Z >-> base_lit.
+Coercion LitBool : bool >-> base_lit.
+
+Coercion App : expr >-> Funclass.
+
+Coercion Val : val >-> expr.
+Coercion Var : string >-> expr.
+
+(** Define some derived forms. *)
+Notation Lam x e := (Rec BAnon x e) (only parsing).
+Notation Let x e1 e2 := (App (Lam x e2) e1) (only parsing).
+Notation Seq e1 e2 := (Let BAnon e1 e2) (only parsing).
+Notation LamV x e := (RecV BAnon x e) (only parsing).
+
+(* No scope for the values, does not conflict and scope is often not inferred
+properly. *)
+Notation "# l" := (LitV l%Z%V%stdpp) (at level 8, format "# l").
+
+Notation "! e" := (Load e%E) (at level 9, right associativity) : expr_scope.
+(* The unicode ← is already part of the notation "_ ← _; _" for bind. *)
+Notation "e1 <- e2" := (Store e1%E e2%E) (at level 80) : expr_scope.
+
+Notation "e1 + e2" := (BinOp PlusOp e1%E e2%E) : expr_scope.
+Notation "e1 - e2" := (BinOp MinusOp e1%E e2%E) : expr_scope.
+Notation "e1 = e2" := (BinOp EqOp e1%E e2%E) : expr_scope.
+
+(* The breaking point '/  ' makes sure that the body of the rec is indented
+by two spaces in case the whole rec does not fit on a single line. *)
+Notation "'rec:' f x := e" := (Rec f%binder x%binder e%E)
+  (at level 200, f at level 1, x at level 1, e at level 200,
+   format "'[' 'rec:'  f  x  :=  '/  ' e ']'") : expr_scope.
+Notation "'rec:' f x := e" := (RecV f%binder x%binder e%E)
+  (at level 200, f at level 1, x at level 1, e at level 200,
+   format "'[' 'rec:'  f  x  :=  '/  ' e ']'") : val_scope.
+Notation "'if:' e1 'then' e2 'else' e3" := (If e1%E e2%E e3%E)
+  (at level 200, e1, e2, e3 at level 200) : expr_scope.
+
+(** Derived notions, in order of declaration. The notations for let and seq
+are stated explicitly instead of relying on the Notations Let and Seq as
+defined above. This is needed because App is now a coercion, and these
+notations are otherwise not pretty printed back accordingly. *)
+Notation "'rec:' f x y .. z := e" := (Rec f%binder x%binder (Lam y%binder .. (Lam z%binder e%E) ..))
+  (at level 200, f, x, y, z at level 1, e at level 200,
+   format "'[' 'rec:'  f  x  y  ..  z  :=  '/  ' e ']'") : expr_scope.
+Notation "'rec:' f x y .. z := e" := (RecV f%binder x%binder (Lam y%binder .. (Lam z%binder e%E) ..))
+  (at level 200, f, x, y, z at level 1, e at level 200,
+   format "'[' 'rec:'  f  x  y  ..  z  :=  '/  ' e ']'") : val_scope.
+
+(* The breaking point '/  ' makes sure that the body of the λ: is indented
+by two spaces in case the whole λ: does not fit on a single line. *)
+Notation "λ: x , e" := (Lam x%binder e%E)
+  (at level 200, x at level 1, e at level 200,
+   format "'[' 'λ:'  x ,  '/  ' e ']'") : expr_scope.
+Notation "λ: x y .. z , e" := (Lam x%binder (Lam y%binder .. (Lam z%binder e%E) ..))
+  (at level 200, x, y, z at level 1, e at level 200,
+   format "'[' 'λ:'  x  y  ..  z ,  '/  ' e ']'") : expr_scope.
+
+Notation "λ: x , e" := (LamV x%binder e%E)
+  (at level 200, x at level 1, e at level 200,
+   format "'[' 'λ:'  x ,  '/  ' e ']'") : val_scope.
+Notation "λ: x y .. z , e" := (LamV x%binder (Lam y%binder .. (Lam z%binder e%E) .. ))
+  (at level 200, x, y, z at level 1, e at level 200,
+   format "'[' 'λ:'  x  y  ..  z ,  '/  ' e ']'") : val_scope.
+
+Notation "'let:' x := e1 'in' e2" := (Lam x%binder e2%E e1%E)
+  (at level 200, x at level 1, e1, e2 at level 200,
+   format "'[' 'let:'  x  :=  '[' e1 ']'  'in'  '/' e2 ']'") : expr_scope.
+Notation "e1 ;; e2" := (Lam BAnon e2%E e1%E)
+  (at level 100, e2 at level 200,
+   format "'[' '[hv' '[' e1 ']' ;;  ']' '/' e2 ']'") : expr_scope.
