tutorial/lithium/primitive_laws.v
@@ -1,0 +1,7 @@
+From iris.program_logic Require Export weakestpre.
+From iris.proofmode Require Import tactics.
+From iris.program_logic Require Import ectx_lifting.
+From lithium.tutorial Require Export notation.
+
+Class tutorialGS (Σ : gFunctors) := {
+}.
